have fully typechecking, axiom-free draft of denotation

theories/AlmostStlc/MrecMonad.v
@@ -25,43 +25,35 @@ Require Import Program.Tactics.
 
 Require Import ITree.Basics.Basics.
 
+Variant void : Set := .
+Global Instance voidEncodedType : EncodedType void := fun v => match v with end.
+
 
 (* could extend to have arbitrary constraints on E, could allow E to include other events*)
 (* universe inconsistenty traces back to here, for now could specialize E to void, perhaps,
    this whole mtree idea was a holdover from when you had more complicated mfix effects *)
 Definition mtree (D : Type) `{EncodedType D} (A : Type) : Type@{entree_u}:= 
-  forall E `(EncodedType E), entree (D + E) A.
+   entree (D + void) A.
 
-Global Instance mtree_monad D `{EncodedType D} : Monad (mtree D) :=
- {|
-   ret := fun _ a E encodes => ret a;
-   bind := fun _ _ m k E encodes => EnTree.bind (m E encodes) (fun a => k a E encodes)
- |}.
+Global Instance mtree_monad D `{EncodedType D} : Monad (mtree D) := Monad_entree.
 
 
-Definition call {D} `{EncodedType D} (d : D) : mtree D (encodes d) :=
-  fun _ _ => trigger d.
+Definition call {D} `{EncodedType D} (d : D) : mtree D (encodes d) := trigger d.
 
-CoFixpoint interp_mtree' {D D' E R} `{EncodedType D} `{EncodedType D'} `{EncodedType E}
-           (bodies : forall (d : D), entree (D + E) (encodes d)) (ot : entree' (D + E) R ) : 
-  entree (D' + E) R :=
+CoFixpoint interp_mtree' {D D' R} `{EncodedType D} `{EncodedType D'}
+           (bodies : forall (d : D), entree (D + void) (encodes d)) (ot : entree' (D + void) R ) : 
+  entree (D' + void) R :=
   match ot with
   | RetF r => Ret r
   | TauF t => Tau (interp_mtree' bodies (observe t))
   | VisF (inl d) k => 
       Tau (interp_mtree' bodies (observe (EnTree.bind (bodies d) k ) ) )
-  | VisF (inr e) k => Vis (@inr D' E e) (fun x => interp_mtree' bodies (observe (k x)))
+  | VisF (inr v) k => Vis (@inr D' void v) (fun x => interp_mtree' bodies (observe (k x)))
   end.
 
-Definition interp_mtree {D D' E R} `{EncodedType D} `{EncodedType D'} `{EncodedType E}
-           (bodies : forall (d : D), entree (D + E) (encodes d)) (t : entree (D + E) R) :
-  entree (D' + E) R := interp_mtree' bodies (observe t).
-
-
-Definition resolve {D D' R} `{EncodedType D} `{EncodedType D'} 
-           (bodies : forall (d : D), mtree D (encodes d)) (m : mtree D R) : mtree D' R :=
-fun E encodes => interp_mtree (fun d => bodies d E encodes) (m E encodes).
-
+Definition interp_mtree {D D' R} `{EncodedType D} `{EncodedType D'}
+           (bodies : forall (d : D), entree (D + void) (encodes d)) (t : entree (D + void) R) :
+  entree (D' + void) R := interp_mtree' bodies (observe t).
 
 
 (* define monad structure*)
