theories/AlmostStlc/Denotation.v
@@ -1,44 +1,16 @@
+Require Export MrecMonad.
+Require Export HeterogeneousRelations.
+Require Export EnTreeDefinition.
+Require Export Syntax.
+From Coq Require Import Lists.List.
+
+From Equations Require Import Equations Signature.
+
+Import Monads.
+Import MonadNotation.
+Local Open Scope monad_scope.
 
 
-Inductive var {T : Type} : T -> list T -> Type := 
-  | VarZ (x : T) l : var x (x :: l)
-  | VarS (x y : T) l : var x l -> var x (y :: l).
-
-
-Inductive type : Type :=
-  | Nat : type
-  | List : type -> type
-                   (* should really be a nonempty list *)
-  | Arrow : type -> list (type * type) -> type -> type
-.
-Notation ctx := (list type).
-Notation rec_ctx := (list (type * type))%type.
-
-
-
-(*TODO : add some basic natural number operations *)
-Inductive term : type -> ctx -> rec_ctx -> Type := 
-  | term_const (n : nat) Γ R : term Nat Γ R
-  | term_nil t Γ R : term (List t) Γ R
-  | term_cons t Γ R (head : term t Γ R) (tail : term (List t) Γ R) : term (List t) Γ R
-  | term_var t Γ R (x : var t Γ) : term t Γ R
-
-  | term_match_nat t Γ R (en : term Nat Γ R) (eZ : term t Γ R) (eS : term t (Nat :: Γ) R ) : term t Γ R
-  | term_match_list t1 t2 Γ R (el : term (List t1) Γ R ) (enil : term t2 Γ R) (econs : term t2 (t1 :: Γ) R) : term t2 Γ R
-  (* might be some subtleties in the application rule you are not sufficiently considering *)
-  | term_app t1 t2 Γ R (e1 : term (Arrow t1 R t2) Γ R) (e2 : term t1 Γ R) : term t2 Γ R
-  (* same here *)
-  | term_abs t1 t2 Γ R R' (e : term t2 (t1 :: Γ) R') : term (Arrow t1 R' t2) Γ R
-  | term_call t1 t2 Γ R (x : var (t1,t2) R) (arg : term t1 Γ R) : term t2 Γ R
-  (* this is the most novel part so be very careful *)
-  | term_mfix t Γ R R' (bodies : mfix_bodies Γ R R) (e : term t Γ R) : term t Γ R'
-
-
-with mfix_bodies : ctx -> rec_ctx -> rec_ctx -> Type := 
-  | mfix_bodies_nil Γ R : mfix_bodies Γ R nil
-  | mfix_bodies_cons Γ R t1 t2 R' (body : term t2 (t1 :: Γ) R) (bodies : mfix_bodies Γ R R') : mfix_bodies Γ R ((t1,t2) :: R')
-.
-(*
 Fixpoint denote_rec_ctx' (R: list (Type * Type) ) : Type@{entree_u} :=
   match R with
   | nil => void
@@ -180,17 +152,3 @@ where denote_bodies (Γ : ctx) (R R' : rec_ctx) (bodies : mfix_bodies Γ R R') (
     denote_bodies Γ' R1 R2 bodies' hyps' arg'.
 Print Assumptions denote_term. (* closed under global context *)
 
-(*one more potential roadblock (might just require equations) need to statically
-  understand the return type of a call *)
-
-(* Fixpoint subst_term t1 t2 Γ R (e : ) *)
-
-
-(*
-TODO: substitution, value, small step semantics
-      mrec monad, denotational semantics
-
-      prove give decode_inject a sane definition (focus on removing the JMeq axiom, which is coming from the usage of dependent induction), move to denotational sep file, find way to test for correctness + 
-*)
-
-*)
